examples/DemoSTLC.v
@@ -1,0 +1,120 @@
+Inductive typ : Set :=
+| TNat
+| TArrow (t1 t2 : typ)
+.
+
+Inductive term : Set :=
+| Var (x : nat)
+| Abs (x : nat) (t : typ) (e : term)
+| App (e1 e2 : term)
+| Const (n : nat)
+.
+
+Inductive value : term -> Prop :=
+| VAbs : forall x t e, value (Abs x t e)
+| VConst : forall n, value (Const n)
+.
+
+From QuickChick Require Import QuickChick.
+
+Require Import Init Arith Logic Bool List.
+Import ListNotations. 
+
+Fixpoint eq_nat (x y : nat) : bool :=
+  match x, y with
+  | 0,0 => true
+  | S x, S y => eq_nat x y
+  | _, _ => false
+  end.
+
+Fixpoint mem (x : nat) (l : list nat) :=
+  match l with
+  | nil => false
+  | (cons y l) => if eq_nat x y then true else mem x l
+  end.
+
+Definition is_free_in (x : nat) (e : term) : bool := 
+  let fix aux (e : term) (env : list nat) : bool :=
+    match e with
+    | Var y => eq_nat x y
+    | Abs y t body => if eq_nat x y then false else aux body (cons y env)
+    | App fe xe => aux fe env || aux xe env  
+    | Const _ => false
+    end in
+  aux e nil.
+
+Definition free_vars (e : term) : list nat :=
+  let fix aux (e : term) (env : list nat) : list nat :=
+    match e with
+    | Var y => if mem y env then nil else cons y nil
+    | Abs y t body => aux body (cons y env)
+    | App fe xe => aux fe env ++ aux xe env
+    | Const _ => nil
+    end in
+  aux e nil.
+
+Definition new_var (l : list nat) : nat := S (list_max l).
+
+Fixpoint subst (x : nat) (v e : term) : term :=
+  match e with
+  | Var y => if eq_nat x y then v else Var y
+  | Abs y t body => if eq_nat x y then Abs y t body else
+                    if is_free_in y v then
+                      let y' := new_var (y :: free_vars v) in
+                      Abs y' t (subst y (Var y') body)
+                    else Abs y t (subst x v body)
+  | App fe xe => App (subst x v fe) (subst x v xe)
+  | Const n => Const n
+  end.
+
+Inductive bigstep : term -> term -> Prop :=
+| big_abs : forall x t e, bigstep (Abs x t e) (Abs x t e)
+| big_app : forall e1 e2 x t body v v',
+  bigstep e1 (Abs x t body) ->
+  bigstep e2 v ->
+  bigstep (subst x v body) v' ->
+  bigstep (App e1 e2) v'
+| big_const : forall n, bigstep (Const n) (Const n)
+.
+
+Inductive env : Set :=
+| enil : env
+| econs : nat -> typ -> env -> env
+.
+
+Inductive bind_typ : env -> nat -> typ -> Prop :=
+| bind_here : forall env v t, bind_typ (econs v t env) v t 
+| bind_later : forall env v t v' t', v <> v' -> bind_typ env v t -> bind_typ (econs v' t' env) v t 
+.
+
+Inductive typing : env -> term -> typ -> Prop :=
+| typ_var : forall x ty g, bind_typ g x ty ->
+                         typing g (Var x) ty
+| typ_abs : forall x t body tbody g, typing (econs x t g) body tbody ->
+                                   typing g (Abs x t body) (TArrow t tbody)
+| typ_app : forall fe xe tfrom tto g, typing g fe (TArrow tfrom tto) ->
+                                    typing g xe tfrom ->
+                                    typing g (App fe xe) tto
+| typ_const : forall n g, typing g (Const n) TNat
+.
+
+
+Instance DecEq_typ : Dec_Eq typ. dec_eq. Defined.
+Instance DeqEq_term : Dec_Eq term. dec_eq. Defined.
+Derive Show for typ.
+Derive Show for term.
+Derive Show for env.
+
+Theorem preservation : forall g e ty e', typing g e ty -> bigstep e e' -> typing g e' ty.
+Proof.
+QuickChickDebug Debug On.  
+schedules.
+valid_schedules.
+quickchick.
+
+
+
+
+
+(*
+Derive Inductive Schedule typing 1 2 derive "Gen" opt "true". Derive Density typing 1 2 derive "Gen". Derive Valid Schedules bind_typ 1 consnum 0 derive "Gen". Locate sized. Check @quickCheck.*)
